src/program_proof/simplepb/pb_leaserenewal_proof.v
@@ -1,0 +1,131 @@
+From Perennial.program_proof Require Import grove_prelude.
+From Goose.github_com.mit_pdos.gokv.simplepb Require Export pb.
+From Perennial.program_proof.simplepb Require Import pb_protocol.
+From Perennial.goose_lang.lib Require Import waitgroup.
+From iris.base_logic Require Export lib.ghost_var mono_nat.
+From iris.algebra Require Import dfrac_agree mono_list.
+From Perennial.program_proof.simplepb Require Import pb_definitions pb_marshal_proof.
+From Perennial.program_proof Require Import marshal_stateless_proof.
+From Perennial.program_proof.reconnectclient Require Import proof.
+From RecordUpdate Require Import RecordSet.
+Import RecordSetNotations.
+
+Section pb_leaserenewal_proof.
+
+Context `{!heapGS Σ}.
+Context {pb_record:Sm.t}.
+Notation OpType := (pb_record.(Sm.OpType)).
+Notation has_op_encoding := (Sm.has_op_encoding pb_record).
+Notation has_snap_encoding := (Sm.has_snap_encoding pb_record).
+Notation compute_reply := (Sm.compute_reply pb_record).
+Notation "server.t" := (server.t (pb_record:=pb_record)).
+Notation pbG := (pbG (pb_record:=pb_record)).
+Notation get_rwops := (get_rwops (pb_record:=pb_record)).
+
+Context `{!pbG Σ}.
+
+Context `{Countable (list (OpType * gname) → iProp Σ)}.
+Context `{config_proof.configG Σ}.
+
+Lemma lease_renewal_step γ γsrv γconf γl newLeaseExpiration st :
+  is_lease config_proof.epochLeaseN γl (config_proof.own_epoch γconf st.(server.epoch)) -∗
+  is_lease_valid_lb γl newLeaseExpiration -∗
+  own_Server_ghost_eph_f st γ γsrv -∗
+  own_Server_ghost_eph_f (st <| server.leaseValid := true |>
+                            <| server.leaseExpiration := newLeaseExpiration |>)
+          γ γsrv
+.
+Proof.
+  iIntros "#Hnew_lease #Hlb".
+  rewrite /own_Server_ghost_eph_f /tc_opaque.
+  iNamed 1.
+  iFrame "∗#%".
+  iNamed "Hlease".
+  iClear "Hlease".
+  repeat iExists _.
+  iFrame "#".
+Qed.
+
+Lemma wp_Server__leaseRenewalThread (s:loc) γ γsrv (epoch:u64) :
+  {{{
+        "#Hsrv" ∷ is_Server s γ γsrv
+  }}}
+    pb.Server__leaseRenewalThread #s #epoch
+  {{{
+        RET #(); True
+  }}}
+.
+Proof.
+  iIntros (?) "H HΦ".
+  iNamed "H".
+  iNamed "Hsrv".
+  wp_lam.
+  iApply (wp_frame_wand with "[HΦ]").
+  { iNamedAccu. }
+  wp_pures.
+  wp_forBreak.
+
+  wp_pures.
+  wp_loadField.
+  wp_apply (config_proof.wp_Clerk__GetLease with "[$HconfCk_is]").
+  iModIntro.
+  iSplit.
+  2: { (* case: got error *)
+    iIntros.
+    wp_pures.
+    wp_if_destruct.
+    2: by exfalso.
+    iModIntro.
+    by iLeft.
+  }
+  (* otherwise, got a lease *)
+  iIntros.
+  wp_pures.
+  wp_loadField.
+  wp_apply (acquire_spec with "[$]").
+  iIntros "[Hlocked Hown]".
+  iNamed "Hown".
+  iNamed "Hvol".
+  wp_loadField.
+  wp_if_destruct.
+  2:{ (* case: epoch mismatch *)
+    wp_loadField.
+    wp_apply (release_spec with "[-]").
+    {
+      iFrame "# Hlocked".
+      iNext.
+      repeat iExists _.
+      iFrame "HghostEph".
+      repeat iExists _.
+      iFrame "∗#%".
+    }
+    wp_pures.
+    iRight.
+    iModIntro.
+    iSplitR; first done.
+    wp_pures.
+    iModIntro.
+    iNamed 1.
+    by iApply "HΦ".
+  }
+  (* case: got lease and the epoch is still the server's epoch *)
+  wp_storeField.
+  wp_storeField.
+  iDestruct (lease_renewal_step with "[$] [$] HghostEph") as "HghostEph".
+  wp_loadField.
+  wp_apply (release_spec with "[-]").
+  {
+    iFrame "# Hlocked".
+    iNext.
+    repeat iExists _.
+    iFrame "HghostEph".
+    repeat iExists _.
+    iFrame "∗#%".
+  }
+  wp_pures.
+  wp_apply (wp_Sleep).
+  wp_pures.
+  by iLeft.
+Qed.
+
+End pb_leaserenewal_proof.
